WIP definition of binary typing

src/Modify.v
@@ -58,23 +58,22 @@ Section parallel.
 
   Definition par_match par (curr : itree (E config) (config * unit)) (rest : list thread)
     : itree (E config) (config * unit) :=
-    (* fun s => *)
-      match (observe curr) with
-      | RetF (s', _) => match rest with
-                       | [] => Ret (s', tt)
-                       | h :: t => Tau (par (h s') t)
-                       end
-      | TauF t => Tau (par t rest)
-      | VisF (inl1 e) k =>
-        match e in modifyE _ C return (C -> itree (E config) (config * unit)) -> _ with
-        | Modify _ f =>
-          fun k' =>
+    match (observe curr) with
+    | RetF (s', _) => match rest with
+                     | [] => Ret (s', tt)
+                     | h :: t => Tau (par (h s') t)
+                     end
+    | TauF t => Tau (par t rest)
+    | VisF (inl1 e) k =>
+      match e in modifyE _ C return (C -> itree (E config) (config * unit)) -> _ with
+      | Modify _ f =>
+        fun k' =>
           '(curr', rest') <- choose k' rest;;
           Vis (inl1 (Modify _ f)) (fun s' => (par (curr' s') rest'))
-        end k
-      | VisF (inr1 e) k =>
-        vis e (fun b => par (k b) rest)
-      end.
+      end k
+    | VisF (inr1 e) k =>
+      vis e (fun b => par (k b) rest)
+    end.
   CoFixpoint par := par_match par.
   Lemma rewrite_par curr rest : par curr rest = par_match par curr rest.
   Proof.
@@ -82,20 +81,6 @@ Section parallel.
     revert curr rest.
     ginit. gcofix CIH. intros. gstep. unfold par. red. reflexivity.
   Qed.
-
-  Lemma par_single :
-    forall t, par t [] = t.
-  Proof.
-    intros. apply bisimulation_is_eq.
-    revert t. pcofix CIH. intros.
-    rewrite rewrite_par. unfold par_match.
-    destruct (observe t) eqn:?; simpl; auto.
-    - destruct r0. pstep. red. rewrite Heqi. simpl. destruct u. constructor; auto.
-    - pstep. red. rewrite Heqi. constructor. right. apply CIH.
-    - destruct e.
-      + destruct m. pstep. unfold choose. unfold choose'.
-        rewritebisim @bind_ret_l.
-  Abort.
 
   (* Not true using ≅, need equivalence that involves nondeterminism: *)
   (* Lemma par_unit : *)
@@ -117,27 +102,31 @@ Section parallel.
   (* Qed. *)
 End parallel.
 
-Variant typing_gen {R} typing (p : perm) (Q : config * R -> Perms) :
-  config -> stateT config (itree (E config)) R -> Prop :=
+(* the config is our last known state *before* giving up control *)
+Variant typing_gen {R} typing (p : perm) (Q : R -> @Perms config) :
+  config -> itree (E config) (R) -> Prop :=
 | typing_gen_ret r c :
     pre p c ->
-    (forall c', rely p c c' -> p ∈ Q (c', r)) ->
-    typing_gen typing p Q c (fun c => Ret (c, r))
+    (* (forall c', rely p c c' -> p ∈ Q (c', r)) -> *)
+    p ∈ Q r ->
+    typing_gen typing p Q c (Ret r)
 | typing_gen_tau t p' c :
+    pre p c ->
     sep_step p p' ->
     typing p' Q c t ->
-    typing_gen typing p Q c (fun c => Tau (t c))
+    typing_gen typing p Q c (Tau t)
 | typing_gen_vis k f p' c :
     pre p c ->
     (forall c, pre p c -> guar p c (f c)) ->
     sep_step p p' ->
-    (forall c', rely p (f c) c' -> typing p' Q c' (k)) ->
-    typing_gen typing p Q c (fun c => Vis (inl1 (Modify _ f)) k)
+    (forall c', rely p (f c) c' -> typing p' Q (f c) (k c')) ->
+    typing_gen typing p Q c (Vis (inl1 (Modify _ f)) k)
 (* (* other events. TODO: generalize E *) *)
 | typing_gen_e X c p' (e : nondetE X) k :
+    pre p c ->
     sep_step p p' ->
-    (forall x, typing p' Q c (fun c => k x)) ->
-    typing_gen typing p Q c (fun c => Vis (inr1 e) k)
+    (forall x, typing p' Q c (k x)) ->
+    typing_gen typing p Q c (Vis (inr1 e) k)
 .
 
 Lemma typing_gen_mon {R} : monotone4 (@typing_gen R).
@@ -148,24 +137,26 @@ Hint Resolve typing_gen_mon : paco.
 
 Definition typing_ {R} := paco4 (@typing_gen R) bot4.
 
-Lemma typing__rely {R} p Q c c' (t : stateT config (itree (E config)) R) :
+Lemma typing__rely {R} p Q c c' (t : itree (E config) (R)) :
   rely p c c' ->
   typing_ p Q c t ->
   typing_ p Q c' t.
 Proof.
   revert p Q c c' t. pcofix CIH. intros p Q c c' t Hrely Ht.
   pinversion Ht; subst.
-  - pstep. constructor. respects. intros. apply H0; auto. etransitivity; eauto.
+  - pstep. constructor. respects. intros. apply H0; auto. (* etransitivity; eauto. *)
   - pstep. econstructor; eauto. right. eapply CIH; eauto. eapply sep_step_rely; eauto.
-  - pstep. econstructor; eauto. right. eapply CIH; eauto. eapply sep_step_rely; eauto.
+  - pstep. econstructor; eauto. right.
     assert (rely p (f c) (f c')) by admit.
     assert (rely p (f c) c'0) by (etransitivity; eauto).
-    specialize (H2 _ H4). pclearbot. apply H2.
+    eapply CIH.
+    + eapply sep_step_rely; eauto. (* apply H1. apply H5. *)
+    + specialize (H2 _ H5). pclearbot. apply H2.
   - pstep. econstructor; eauto. right. eapply CIH; eauto. eapply sep_step_rely; eauto.
-    apply H0.
+    apply H1.
 Admitted.
 
-Lemma typing__lte {R} p Q Q' c (t : stateT config (itree (E config)) R) :
+Lemma typing__lte {R} p Q Q' c (t : itree (E config) R) :
   typing_ p Q c t ->
   (forall r, Q r ⊨ Q' r) ->
   typing_ p Q' c t.
@@ -174,7 +165,7 @@ Proof.
   pstep. pinversion Htyping; pclearbot; subst; econstructor; eauto.
   - intros. apply Hlte; eauto.
   - intros. specialize (H2 _ H3). pclearbot. eauto.
-  - intros. specialize (H0 x). eauto.
+  - intros. specialize (H1 x). eauto.
 Qed.
 
 (* Lemma typing__lte' p p' Q c (t : itree (E config) (config * unit)) : *)
@@ -191,7 +182,7 @@ Qed.
 
 (* Definition typing {R} P Q (t : stateT config (itree (E config)) R) := *)
 (*   forall p c, p ∈ P -> pre p c -> typing_ p Q (t c). *)
-Definition typing {R} P Q (t : stateT config (itree (E config)) R) :=
+Definition typing {R} P Q (t : itree (E config) R) :=
   forall p c, p ∈ P -> pre p c -> typing_ p Q c t.
 
 Lemma typing_lte {R} P P' (Q Q' : config * R -> Perms) t: (* (t : stateT config (itree (E config)) R) : *)
@@ -204,137 +195,148 @@ Proof.
 Qed.
 
 Lemma typing__bind {R S} p Q1 Q2 c
-      (t1 : stateT config (itree (E config)) R)
-      (t2 : R -> stateT config (itree (E config)) S)
+      (t1 : itree (E config) R)
+      (t2 : R -> itree (E config) S)
       r' :
   typing_ p Q1 c t1 ->
-  (forall r p c, (forall c', rely p c c' -> p ∈ Q1 (c', r)) ->
+  (forall r p c, p ∈ Q1 r ->
             pre p c ->
             paco4 typing_gen r' p Q2 c (t2 r)) ->
-  paco4 typing_gen r' p Q2 c (fun c => x <- t1 c;; t2 (snd x) (fst x)).
+  paco4 typing_gen r' p Q2 c (bind t1 t2).
 Proof.
   revert p Q1 Q2 c t1 t2. pcofix CIH. intros p Q1 Q2 c t1 t2 Ht1 Ht2.
   pinversion Ht1; subst.
-  - assert ((fun c0 => x <- Ret (c0, r0);; t2 (snd x) (fst x)) = (t2 r0)).
-    { apply functional_extensionality. intros. rewritebisim @bind_ret_l. auto. }
-    rewrite H1.
+  - rewritebisim @bind_ret_l.
     eapply paco4_mon; eauto.
-  - assert ((fun c0 : config => x <- Tau (t c0);; t2 (snd x) (fst x)) =
-            (fun c0 => Tau (x <- (t c0);; t2 (snd x) (fst x)))).
-    { apply functional_extensionality. intros. rewritebisim @bind_tau. auto. }
-    rewrite H1. pstep. econstructor; eauto.
-  - assert ((fun _ : config => x <- Vis (inl1 (Modify config f)) k;; t2 (snd x) (fst x)) =
-            (fun _ => Vis (inl1 (Modify config f)) (fun s => x <- k s;; t2 (snd x) (fst x)))).
-    { apply functional_extensionality. intros. rewritebisim @bind_vis. auto. }
-    rewrite H3. pstep. econstructor; eauto. intros.
+  - rewritebisim @bind_tau.
+    pstep. econstructor; eauto. right. eapply CIH; eauto.
+  - rewritebisim @bind_vis. pstep. econstructor; eauto. intros.
     right. eapply CIH; eauto.
-    specialize (H2 _ H4). pclearbot. apply H2.
-  - assert ((fun _ : config => x <- Vis (inr1 e) k;; t2 (snd x) (fst x)) =
-            (fun _ => Vis (inr1 e) (fun x => x <- k x;; t2 (snd x) (fst x)))).
-    { apply functional_extensionality. intros. rewritebisim @bind_vis. auto. }
-    rewrite H1. pstep. econstructor; eauto. intros.
-    right. eapply CIH; eauto. apply H0.
+    specialize (H2 _ H3). pclearbot. apply H2.
+  - rewritebisim @bind_vis. pstep. econstructor; eauto. intros.
+    right. eapply CIH; eauto. apply H1.
 Qed.
 
 Lemma typing_bind {R S} P Q1 Q2
-      (t1 : stateT config (itree (E config)) R)
-      (t2 : R -> stateT config (itree (E config)) S) :
+      (t1 : itree (E config) R)
+      (t2 : R -> itree (E config) S) :
   typing P Q1 t1 ->
-  (forall c r, typing (Q1 (c, r)) Q2 (t2 r)) ->
+  (forall r, typing (Q1 r) Q2 (t2 r)) ->
   typing P Q2 (bind t1 t2).
 Proof.
   intros Ht1 Ht2 p c Hp Hpre.
-  eapply typing__bind; eauto. intros. eapply Ht2; eauto. apply H; reflexivity.
+  eapply typing__bind; eauto. (* intros. eapply Ht2; eauto. apply H; reflexivity. *)
 Qed.
 
-Lemma typing__tau {R} p (Q : config * R -> Perms) c t :
+Lemma typing__tau {R} p (Q : R -> Perms) c t :
   typing_ p Q c t ->
-  typing_ p Q c (fun c => Tau (t c)).
+  typing_ p Q c (Tau t).
 Proof.
   intros Ht.
   pinversion Ht; subst; simpl; try solve [pstep; econstructor; try reflexivity; eauto].
 Qed.
+
+(* Lemma typing__par_empty p Q c t : *)
+(*   typing_ p Q c t -> *)
+(*   typing_ p Q c (par t []). *)
+(* Proof. *)
+(*   revert p t c. *)
+(*   pcofix CIH. *)
+(*   intros p t c Ht. *)
+(*   rewrite rewrite_par. unfold par_match. *)
+(*   pinversion Ht; subst; simpl. *)
+(*   - destruct r0. pstep. constructor; auto. *)
+(*   - pstep. econstructor; eauto. (* right. eapply CIH; eauto. *) *)
+(*   - pstep. unfold choose, choose'. *)
+(*     assert ((fun _ : config => x_ <- Ret (k, []);; let (curr', rest') := x_ in Vis (inl1 (Modify config f)) (fun s' => par curr' rest' s')) = *)
+(*             (fun _ => Vis (inl1 (Modify config f)) (fun s' => par k [] s'))). *)
+(*     { apply functional_extensionality. intros. *)
+(*       rewritebisim @bind_ret_l. reflexivity. } *)
+(*     unfold thread, stateT in H4. rewrite H4. *)
 
 (* TODO after this point *)
 Lemma typing__par_empty p Q c t :
   typing_ p Q c t ->
   typing_ p Q c (par t []).
 Proof.
-  revert p t.
+  revert p t c.
   pcofix CIH.
-  intros p t Ht. rewrite rewrite_par. unfold par_match.
+  intros p t c Ht.
+  rewrite rewrite_par. unfold par_match.
   pinversion Ht; subst; simpl.
-  - destruct r0. pstep. constructor; auto.
-  - pstep. econstructor; eauto.
-  - pstep. unfold choose, choose'. rewritebisim @bind_ret_l.
+  - destruct r0, u. pstep. constructor; auto.
+  - pstep. econstructor; eauto. (* right. eapply CIH; eauto. *)
+  - pstep. unfold choose, choose'.
+    rewritebisim @bind_ret_l.
     econstructor; eauto.
     clear Ht H.
     right. eapply CIH; eauto.
-    specialize (H1 _ _ H H2). pclearbot. eauto.
-  - pstep. econstructor; eauto. intros. right. apply CIH. apply H0.
+    specialize (H2 _ H). pclearbot. eauto.
+  - pstep. econstructor; eauto. intros. right. apply CIH. apply H1.
 Qed.
 
 Lemma typing_par_empty P Q t :
   typing P Q t ->
   typing P Q (par t []).
 Proof.
-  intros Ht p Hp. apply typing__par_empty; auto.
+  intros Ht p c Hp Hpre. apply typing__par_empty; auto.
 Qed.
 
-Lemma typing__frame p p' r (Q : config * unit -> Perms) R t c :
-  typing_ p Q (t c) ->
+Lemma typing__frame p p' r (Q : unit -> Perms) R c t :
+  typing_ p Q c t ->
   r ∈ R ->
   p ** r <= p' ->
   pre p' c ->
-  typing_ p' (fun c' => Q c' * R) (t c).
+  typing_ p' (fun c' => Q c' * R) c t.
 Proof.
-(*   revert p p' r Q R t c. *)
-(*   pcofix CIH. intros p p' r' Q R t c Ht Hr Hp' Hpre. *)
-(*   pinversion Ht; subst. *)
-(*   - destruct r0. pstep. constructor; auto. *)
-(*     apply Hp'. *)
-(*     eapply Perms_upwards_closed; eauto. apply sep_conj_Perms_perm; auto. *)
-(*     apply H0; auto. apply Hp'; auto. *)
-(*   - pstep. econstructor; auto. *)
-(*     + eapply sep_step_lte; eauto. eapply sep_step_sep_conj_l. *)
-(*       apply Hp' in Hpre. apply Hpre. *)
-(*       apply H0. *)
-(*     + right. eapply CIH; eauto. reflexivity. *)
-(*       split; [| split]. pinversion H1; auto. *)
-(*       apply Hp'. apply Hpre. *)
-(*       apply H0. apply Hp' in Hpre. apply Hpre. *)
-(*   - pstep. econstructor; auto. *)
-(*     + apply Hp'. constructor. left. auto. *)
-(*     + eapply sep_step_lte; eauto. eapply sep_step_sep_conj_l. *)
-(*       apply Hp' in Hpre. apply Hpre. *)
-(*       apply H1. *)
-(*     + intros. right. *)
-(*       assert (rely p c' c''). *)
-(*       { apply Hp'. auto. } *)
-(*       specialize (H2 _ H4). pclearbot. *)
-(*       eapply CIH; eauto. reflexivity. *)
-(*       split; [| split]. *)
-(*       * pinversion H2; auto. *)
-(*       * pose proof Hpre as Hpre'. apply Hp' in Hpre'. destruct Hpre' as (_ & _ & Hsep). *)
-(*         apply Hsep in H0. respects. etransitivity; eauto. apply Hp'. auto. apply Hp'; auto. *)
-(*       * apply H1. apply Hp' in Hpre. apply Hpre. *)
-(*   - pstep. econstructor; eauto. *)
-(*     + eapply sep_step_lte; eauto. eapply sep_step_sep_conj_l. *)
-(*       apply Hp' in Hpre. apply Hpre. *)
-(*       apply H0. *)
-(*     + intros. specialize (H1 x). right. eapply CIH; eauto. reflexivity. *)
-(*       split; [| split]. pinversion H1; auto. *)
-(*       apply Hp'. auto. *)
-(*       apply Hp' in Hpre. apply H0. apply Hpre. *)
-(* Qed. *)
-Abort.
+  revert p p' r Q R t c.
+  pcofix CIH. intros p p' r' Q R t c Ht Hr Hp' Hpre.
+  pinversion Ht; subst.
+  - destruct r0. pstep. constructor; auto.
+    (* apply Hp'. *)
+    eapply Perms_upwards_closed; eauto. apply sep_conj_Perms_perm; auto.
+    (* apply H0; auto. apply Hp'; auto. *)
+  - pstep. econstructor; auto.
+    + eapply sep_step_lte; eauto. eapply sep_step_sep_conj_l.
+      apply Hp' in Hpre. apply Hpre.
+      apply H0.
+    + right. eapply CIH; eauto. reflexivity.
+      split; [| split]. pinversion H1; auto.
+      apply Hp'. apply Hpre.
+      apply H0. apply Hp' in Hpre. apply Hpre.
+  - pstep. econstructor; auto.
+    (* + apply Hp'. constructor. left. auto. *)
+    + intros. apply Hp'. constructor. left. apply H0. apply Hp'; auto.
+    + eapply sep_step_lte; eauto. eapply sep_step_sep_conj_l.
+      apply Hp' in Hpre. apply Hpre.
+      apply H1.
+    + intros. right.
+      assert (rely p (f c) c').
+      { apply Hp'. auto. }
+      specialize (H2 _ H4). pclearbot.
+      eapply CIH; eauto. reflexivity.
+      split; [| split].
+      * pinversion H2; auto.
+      * pose proof Hpre as Hpre'. apply Hp' in Hpre'. destruct Hpre' as (Hp & Hr' & Hsep).
+        specialize (H0 _ Hp). apply Hsep in H0. respects. (* etransitivity; eauto. apply Hp'. auto. apply Hp'; auto. *)
+      * apply H1. apply Hp' in Hpre. apply Hpre.
+  - pstep. econstructor; eauto.
+    + eapply sep_step_lte; eauto. eapply sep_step_sep_conj_l.
+      apply Hp' in Hpre. apply Hpre.
+      apply H0.
+    + intros. specialize (H1 x). right. eapply CIH; eauto. reflexivity.
+      split; [| split]. pinversion H1; auto.
+      apply Hp'. auto.
+      apply Hp' in Hpre. apply H0. apply Hpre.
+Qed.
 
-(* Lemma typing__frame' p p' r (Q R : config * unit -> Perms) t c : *)
-(*   typing_ p Q c t -> *)
-(*   (forall c', rely r c c' -> r ∈ R (c', tt)) -> *)
-(*   r ** p <= p' -> *)
-(*   pre p' c -> *)
-(*   typing_ p' (fun c => R c * Q c) c t. *)
+Lemma typing__frame' p p' r (Q R : (config * unit) -> Perms) t c :
+  typing_ p Q c t ->
+  (forall c', rely r c c' -> r ∈ R (c', tt)) ->
+  r ** p <= p' ->
+  pre p' c ->
+  typing_ p' (fun c => R c * Q c) c t.
+Admitted.
 (* Proof. *)
 (*   revert p p' r Q R t c. *)
 (*   pcofix CIH. intros p p' r' Q R t c Ht Hr Hp' Hpre. *)
@@ -386,56 +388,41 @@ Abort.
 (*       destruct Hpre as (_ & _ & Hpre). symmetry in Hpre. apply Hpre. *)
 (* Qed. *)
 
-Lemma typing_frame P P' (Q : config * unit -> Perms) t :
-  typing P Q t ->
-  typing (P * P') (fun r => Q r * P') t.
-Proof.
-  intros Ht p'' (p & p' & Hp & Hp' & Hlte).
-  specialize (Ht _ Hp).
-  revert Ht Hp Hp' Hlte. revert P P' Q t p p'' p'.
-  pcofix CIH. intros. pinversion Ht; subst; simpl.
-  - destruct r0. pstep. constructor; auto.
-    admit.
-    intros. eapply Perms_upwards_closed; eauto.
-    apply sep_conj_Perms_perm; auto. apply H0. apply Hlte; auto.
-  - pstep. econstructor; auto.
-    + eapply sep_step_lte; eauto. eapply sep_step_sep_conj_l.
-      apply Hp' in Hpre. apply Hpre.
-      apply H0.
+(* Lemma typing_frame P P' (Q : config * unit -> Perms) t : *)
+(*   typing P Q t -> *)
+(*   typing (P * P') (fun r => Q r * P') t. *)
+(* Proof. *)
+(*   intros Ht p'' c (p & p' & Hp & Hp' & Hlte) Hpre. *)
+(*   specialize (Ht _ _ Hp). *)
+(*   revert Ht Hp Hp' Hlte. revert P P' Q t p p'' p'. *)
+(*   pcofix CIH. intros. pinversion Ht; subst; simpl. *)
+(*   - destruct r0. pstep. constructor; auto. *)
+(*     admit. *)
+(*     intros. eapply Perms_upwards_closed; eauto. *)
+(*     apply sep_conj_Perms_perm; auto. apply H0. apply Hlte; auto. *)
+(*   - pstep. econstructor; auto. *)
+(*     + eapply sep_step_lte; eauto. eapply sep_step_sep_conj_l. *)
+(*       apply Hp' in Hpre. apply Hpre. *)
+(*       apply H0. *)
 
-    2: {
-      right. eapply CIH; eauto.
+(*     2: { *)
+(*       right. eapply CIH; eauto. *)
 
-    eapply typing__frame; eauto. apply H; auto. apply H3. auto.
-Qed.
-
-Lemma typing_rely p (Q : config * unit -> Perms) t c c' :
-  rely p c c' ->
-  typing_ p Q c t ->
-  typing_ p Q c' t.
-Proof.
-  revert p Q c c' t. pcofix CIH.
-  intros p Q c c' t Hrely Ht. pinversion Ht; subst; simpl.
-  - pstep. admit.
-  - pstep. (* econstructor; eauto. right. eapply CIH; eauto. eapply sep_step_rely; eauto. *)
-    admit.
-  - pstep. econstructor. respects. admit. apply H1. intros. right. eapply CIH.
-    reflexivity. admit.
-  -
-Abort.
+(*     eapply typing__frame; eauto. apply H; auto. apply H3. auto. *)
+(* Qed. *)
 
 Lemma typing__par p1 p2 p Q1 Q2 c t1 t2 :
-  typing_ p1 Q1 c (t1 c) ->
+  typing_ p1 Q1 c t1 ->
   typing_ p2 Q2 c (t2 c) ->
   p1 ** p2 <= p ->
   pre p c ->
-  typing_ p (fun c => Q1 c * Q2 c) c (par t1 [t2] c).
+  typing_ p (fun c => Q1 c * Q2 c) c (par t1 [t2]).
 Proof.
   revert p1 p2 p c t1 t2. pcofix CIH. intros p1 p2 p c t1 t2 Ht1 Ht2 Hlte Hpre.
   rewrite rewrite_par. unfold par_match.
   (* assert (Hguar1: guar p1 c c) by reflexivity. specialize (Ht1 _ Hguar1). *)
   pinversion Ht1; subst; simpl.
-  - destruct r0. pstep. econstructor; eauto. reflexivity. left.
+  - destruct r0, u. pstep. econstructor; eauto. reflexivity. left.
     eapply paco4_mon_bot; eauto. eapply typing__frame'; eauto.
     apply typing__par_empty. apply Ht2; intuition.
     intros; eauto.
