src/ITreeDefinition.v
@@ -1,0 +1,432 @@
+(** * Interaction trees: core definitions *)
+
+(* begin hide *)
+Require Import ExtLib.Structures.Functor.
+Require Import ExtLib.Structures.Applicative.
+Require Import ExtLib.Structures.Monad.
+Require Import Program.Tactics.
+
+From Coq Require Import
+     JMeq.
+
+From Paco Require Import paco.
+
+Set Implicit Arguments.
+Set Contextual Implicit.
+Set Primitive Projections.
+(* end hide *)
+
+(** ** The type of interaction trees *)
+
+(** An [itree E R] is the denotation of a program as coinductive
+    (possibly infinite) tree where the leaves [Ret] are labeled with
+    [R] and every node is either a [Tau] node with one child, or a
+    branching node [Vis] with a _visible event_ [E X] that branches
+    on the values of [X]. *)
+
+Section itree.
+
+  Context {E : Type -> Type} {R : Type}.
+
+  (** The type [itree] is defined as the final coalgebra ("greatest
+      fixed point") of the functor [itreeF]. *)
+  Variant itreeF (itree : Type) :=
+  | RetF (r : R)
+  | TauF {X : Type} (t : X -> itree)
+  | VisF {X : Type} (e : E X) (k : X -> itree)
+  .
+
+  (** We define non-recursive types such as [itreeF] using the [Variant]
+      command. The main practical difference from [Inductive] is that
+      [Variant] does not generate any induction schemes (which are
+      unnecessary). *)
+
+  CoInductive itree : Type := go
+  { _observe : itreeF itree }.
+
+  (** A primitive projection, such as [_observe], must always be
+      applied. To be used as a function, wrap it explicitly:
+      [fun x => _observe x] or [observe] (defined below). *)
+
+  (* Notes about using [itree]:
+
+     - You should simplify using [cbn] rather than [simpl] when working
+       with terms of the form [observe e] where [e] is defined by
+       [CoFixpoint] (as in [bind] and [map] below).  [simpl] does not
+       unfold the definition properly to expose the [observe t] term.
+
+     - Once you have [observe t] as the subject of [match], you can
+       [destruct (observe t)] to do the case split.
+   *)
+
+End itree.
+
+(* begin hide *)
+(*
+  The following line removes the warning on >=8.10, but is incompatible for <8.10
+ *)
+(* Declare Scope itree_scope. *)
+Bind Scope itree_scope with itree.
+Delimit Scope itree_scope with itree.
+Local Open Scope itree_scope.
+
+Arguments itree _ _ : clear implicits.
+Arguments itreeF _ _ : clear implicits.
+(* end hide *)
+
+(** An [itree'] is a "forced" [itree]. It is the type of inputs
+    of [go], and outputs of [observe]. *)
+Notation itree' E R := (itreeF E R (itree E R)).
+
+(** We wrap the primitive projection [_observe] in a function
+    [observe]. *)
+Definition observe {E R} (t : itree E R) : itree' E R := @_observe E R t.
+
+(** Note that when [_observe] appears unapplied in an expression,
+    it is implicitly wrapped in a function. However, there is no
+    way to distinguish whether such wrapping took place, so relying
+    on this behavior can lead to confusion.
+
+    We recommend to always use a primitive projection applied,
+    and wrap it in a function explicitly like the above to pass
+    around as a first-order function. *)
+
+(** We introduce notation for the [Tau], [Ret], and [Vis] constructors. Using
+    notation rather than definitions works better for extraction.  (The [spin]
+    definition, given below does not extract correctly if [Tau] is a definition.)
+
+    Using this notation means that we occasionally have to eta expand, e.g.
+    writing [Vis e (fun x => Ret x)] instead of [Vis e Ret]. (In this
+    particular case, this is [ITree.trigger].)
+*)
+Notation Ret x := (go (RetF x)).
+Notation Tau t := (go (TauF t)).
+Notation Vis e k := (go (VisF e k)).
+
+(** ** Main operations on [itree] *)
+
+(** The core definitions are wrapped in a module for namespacing.
+    They are meant to be used qualified (e.g., ITree.bind) or
+    via notations (e.g., [>>=]). *)
+
+(** *** How to write cofixpoints *)
+
+(** We define cofixpoints in two steps: first a plain definition
+    (prefixed with an [_], e.g., [_bind], [_iter]) defines the body
+    of the function:
+
+    - it takes the recursive call ([bind]) as a parameter;
+    - if we are deconstructing an itree, this body takes
+      the unwrapped [itreeF];
+
+    second the actual [CoFixpoint] (or, equivalently, [cofix]) ties
+    the knot, applying [observe] to any [itree] parameters. *)
+
+(** This style allows us to keep [cofix] from ever appearing in
+    proofs, which could otherwise get quite unwieldly.
+    For every [CoFixpoint] (such as [bind]), we prove an unfolding
+    lemma to rewrite it as a term whose head is [_bind], without
+    any [cofix] above it.
+[[
+    unfold_bind : observe (bind t k)
+                = observe (_bind (fun t' => bind t' k) t)
+]]
+    Note that this is an equality "up to" [observe]. It would not be
+    provable if it were a plain equality:
+[[
+    bind t k = _bind (...) t  (* unfold the definition of [bind]... *)
+    (cofix bind' t1 := _bind (...) t1) t = _bind (...) t1
+]]
+    The [cofix] is stuck, and can only be unstuck under the primitive
+    projection [_observe] (which is wrapped by [observe]).
+ *)
+
+(** *** Definitions *)
+
+(** These are meant to be imported qualified, e.g., [ITree.bind],
+    [ITree.trigger], to avoid ambiguity with identifiers of the same
+    name (some of which are overloaded generalizations of these).
+ *)
+Module ITree.
+
+(** [bind]: monadic composition, tree substitution, sequencing of
+    computations. [bind t k] is also denoted by [t >>= k] and using
+    "do-notation" [x <- t ;; k x]. *)
+
+Section bind.
+  Context {E : Type -> Type} {T U : Type}.
+  (* We can keep the continuation outside the cofixpoint.
+     In particular, this allows us to nest [bind] in other cofixpoints,
+     as long as the recursive occurences are in the continuation
+     (i.e., this makes it easy to define tail-recursive functions).
+   *)
+  Variable k : T -> itree E U.
+
+  Definition _bind
+             (bind : itree E T -> itree E U)
+             (oc : itreeF E T (itree E T)) : itree E U :=
+    match oc with
+    | RetF r => k r
+    | TauF t => Tau (fun x => bind (t x))
+    | VisF e h => Vis e (fun x => bind (h x))
+    end.
+
+  CoFixpoint bind' (t : itree E T) : itree E U :=
+    _bind bind' (observe t).
+
+End bind.
+
+Arguments _bind _ _ /.
+
+
+Notation bind c k := (bind' k c).
+
+
+(** Monadic composition of continuations (i.e., Kleisli composition).
+ *)
+Definition cat {E T U V}
+           (k : T -> itree E U) (h : U -> itree E V) :
+  T -> itree E V :=
+  fun t => bind' h (k t).
+
+(** [iter]: See [Basics.Basics.MonadIter]. *)
+
+(* [on_left lr l t]: run a computation [t] if the first argument is an [inl l].
+   [l] must be a variable (used as a pattern), free in the expression [t]:
+   - [on_left (inl x) l t = t{l := x}]
+   - [on_left (inr y) l t = Ret y]
+ *)
+Notation on_left lr l t :=
+  (match lr with
+  | inl l => t
+  | inr r => Ret r
+  end) (only parsing).
+
+(* Note: here we must be careful to call [iter_ l] under [Tau] to avoid an eager
+   infinite loop if [step i] is always of the form [Ret (inl _)] (cf. issue #182). *)
+Definition iter {E : Type -> Type} {R I: Type}
+           (step : I -> itree E (I + R)) : I -> itree E R :=
+  cofix iter_ i := bind (step i) (fun lr => on_left lr l (Tau (fun _ : unit => iter_ l))).
+
+(* note(gmm): There needs to be generic automation for monads to simplify
+ * using the monad laws up to a setoid.
+ * this would be *really* useful to a lot of projects.
+ *
+ * this will be especially important for this project because coinductives
+ * don't simplify very nicely.
+ *)
+
+(** Functorial map ([fmap] in Haskell) *)
+Definition map {E R S} (f : R -> S)  (t : itree E R) : itree E S :=
+  bind t (fun x => Ret (f x)).
+
+(** Atomic itrees triggering a single event. *)
+Definition trigger {E : Type -> Type} : forall X, E X -> itree E X :=
+  fun R e => Vis e (fun x => Ret x).
+
+(** Ignore the result of a tree. *)
+Definition ignore {E R} : itree E R -> itree E unit :=
+  map (fun _ => tt).
+
+(** Infinite taus. *)
+CoFixpoint spin {E R} : itree E R := Tau (fun _ : unit => spin).
+
+(** Repeat a computation infinitely. *)
+Definition forever {E R S} (t : itree E R) : itree E S :=
+  cofix forever_t := bind t (fun _ => Tau (fun _ : unit => forever_t)).
+
+End ITree.
+
+(** ** Notations *)
+
+(** Sometimes it's more convenient to work without the type classes
+    [Monad], etc. When functions using type classes are specialized,
+    they simplify easily, so lemmas without classes are easier
+    to apply than lemmas with.
+
+    We can also make ExtLib's [bind] opaque, in which case it still
+    doesn't hurt to have these notations around.
+ *)
+
+Module ITreeNotations.
+Notation "t1 >>= k2" := (ITree.bind t1 k2)
+  (at level 58, left associativity) : itree_scope.
+Notation "x <- t1 ;; t2" := (ITree.bind t1 (fun x => t2))
+  (at level 61, t1 at next level, right associativity) : itree_scope.
+Notation "` x : t <- t1 ;; t2" := (ITree.bind t1 (fun x : t => t2))
+  (at level 61, t at next level, t1 at next level, x ident, right associativity, only parsing) : itree_scope.
+Notation "t1 ;; t2" := (ITree.bind t1 (fun _ => t2))
+  (at level 61, right associativity) : itree_scope.
+Notation "' p <- t1 ;; t2" :=
+  (ITree.bind t1 (fun x_ => match x_ with p => t2 end))
+  (at level 61, t1 at next level, p pattern, right associativity) : itree_scope.
+Infix ">=>" := ITree.cat (at level 61, right associativity) : itree_scope.
+End ITreeNotations.
+
+(** ** Instances *)
+
+Instance Functor_itree {E} : Functor (itree E) :=
+{ fmap := @ITree.map E }.
+
+(* Instead of [pure := @Ret E], [ret := @Ret E], we eta-expand
+   [pure] and [ret] to make the extracted code respect OCaml's
+   value restriction. *)
+Instance Applicative_itree {E} : Applicative (itree E) :=
+{ pure := fun _ x => Ret x
+; ap := fun _ _ f x =>
+          ITree.bind f (fun f => ITree.bind x (fun x => Ret (f x)))
+}.
+
+Instance Monad_itree {E} : Monad (itree E) :=
+{| ret := fun _ x => Ret x
+;  bind := fun T U t k => @ITree.bind' E T U k t
+|}.
+
+(** ** Tactics *)
+
+(* [inv], [rewrite_everywhere], [..._except] are general purpose *)
+
+Lemma hexploit_mp: forall P Q: Type, P -> (P -> Q) -> Q.
+Proof. intuition. Defined.
+Ltac hexploit x := eapply hexploit_mp; [eapply x|].
+
+Tactic Notation "hinduction" hyp(IND) "before" hyp(H)
+  := move IND before H; revert_until IND; induction IND.
+
+Ltac inv H := inversion H; clear H; subst.
+
+Ltac rewrite_everywhere lem :=
+  progress ((repeat match goal with [H: _ |- _] => rewrite lem in H end); repeat rewrite lem).
+
+Ltac rewrite_everywhere_except lem X :=
+  progress ((repeat match goal with [H: _ |- _] =>
+                 match H with X => fail 1 | _ => rewrite lem in H end
+             end); repeat rewrite lem).
+
+Ltac genobs x ox := remember (observe x) as ox.
+Ltac genobs_clear x ox := genobs x ox; match goal with [H: ox = observe x |- _] => clear H x end.
+Ltac simpobs := repeat match goal with [H: _ = observe _ |- _] =>
+                    rewrite_everywhere_except (@eq_sym _ _ _ H) H
+                end.
+
+Section eqit.
+  Context {E : Type -> Type} {R1 R2 : Type} (RR : R1 -> R2 -> Prop).
+
+  Inductive refF (ref : itree E R1 -> itree E R2 -> Prop) :
+    itree' E R1 -> itree' E R2 -> Prop :=
+  | EqRet r1 r2
+          (REL: RR r1 r2):
+      refF ref (RetF r1) (RetF r2)
+  | EqTau {X1 X2} m1 m2
+          (REL: forall (x1 : X1), exists (x2 : X2), ref (m1 x1) (m2 x2)):
+      refF ref (TauF m1) (TauF m2)
+  | EqVis {u} (e : E u) k1 k2
+          (REL: forall v, ref (k1 v) (k2 v) : Prop):
+      refF ref (VisF e k1) (VisF e k2)
+  | EqTauL {X} t1 ot2
+           (REL: forall (x : X), refF ref (observe (t1 x)) ot2):
+      refF ref (TauF t1) ot2
+  | EqTauR {X} ot1 t2 (x : X)
+           (REL: refF ref ot1 (observe (t2 x))):
+      refF ref ot1 (TauF t2)
+  .
+  Hint Constructors refF: core.
+
+
+  Definition ref_ ref :
+    itree E R1 -> itree E R2 -> Prop :=
+    fun t1 t2 => refF ref (observe t1) (observe t2).
+  Hint Unfold ref_: core.
+
+  Lemma refF_mono x0 x1 ref ref'
+        (IN: refF ref x0 x1)
+        (LE: ref <2= ref'):
+    refF ref' x0 x1.
+  Proof.
+    intros. induction IN; eauto.
+    econstructor; eauto. intros. destruct (REL x1). exists x. eauto.
+  Qed.
+
+  Lemma ref__mono : monotone2 ref_.
+  Proof.
+    do 2 red. intros. eapply refF_mono; eauto.
+  Qed.
+
+  Hint Resolve ref__mono : paco.
+
+  Definition ref : itree E R1 -> itree E R2 -> Prop :=
+    paco2 ref_ bot2.
+
+End eqit.
+
+
+
+(* This exists in the stdlib as [ProofIrrelevance.inj_pair2], but we reprove
+   it to not depend on proof irrelevance (we use axiom [JMeq.JMeq_eq] instead) *)
+Lemma inj_pair2 :
+  forall (U : Type) (P : U -> Type) (p : U) (x y : P p),
+    existT P p x = existT P p y -> x = y.
+Proof.
+  intros. apply JMeq_eq.
+  refine (
+      match H in _ = w return JMeq x (projT2 w) with
+      | eq_refl => JMeq_refl
+      end).
+Qed.
+
+Lemma ref_refl {E R} (t : itree E R) : ref eq t t.
+Proof.
+  revert t. pcofix CIH.
+  pstep. red. intros t. destruct (observe t); try constructor; auto.
+  intros x. exists x. right. auto.
+Qed.
+
+Goal forall {E}, ref eq (Ret 1 : itree E nat) (Tau (fun b : bool => if b then Ret 1 else Ret 2)).
+Proof.
+  intros. pstep. red. apply EqTauR with (x := true).
+  constructor; auto.
+Qed.
+
+Goal forall {E}, ~ ref eq (Tau (fun b : bool => if b then Ret 1 else Ret 2)) (Ret 1 : itree E nat).
+Proof.
+  intros ? ?. pinversion H. 2: { (* todo *) apply ref__mono. }.
+  clear H; subst. apply inj_pair2 in H2. subst. specialize (REL false).
+  inversion REL. inversion REL0.
+Qed.
+
+Variant test : Type -> Type :=
+| Event : nat -> test unit
+.
+
+Goal ref eq
+     (Tau (fun b : bool => if b then Vis (Event 1) (fun _ => Ret 1) else Vis (Event 1) (fun _ => Ret 2)))
+     (Vis (Event 1) (fun _ => Tau (fun b : bool => if b then Ret 1 else Ret 2))).
+Proof.
+  pstep. constructor. intros [].
+  - constructor. intros. left. pstep. apply EqTauR with (x := true). constructor; auto.
+  - constructor. intros. left. pstep. apply EqTauR with (x := false). constructor; auto.
+Qed.
+
+Goal ~ ref eq
+     (Vis (Event 1) (fun _ => Tau (fun b : bool => if b then Ret 1 else Ret 2)))
+     (Tau (fun b : bool => if b then Vis (Event 1) (fun _ => Ret 1) else Vis (Event 1) (fun _ => Ret 2))).
+Proof.
+  intro. pinversion H. 2: apply ref__mono.
+  apply inj_pair2 in H3. clear H; subst. destruct x.
+  - inversion REL; clear REL.
+    apply inj_pair2 in H1.
+    apply inj_pair2 in H2.
+    apply inj_pair2 in H.
+    apply inj_pair2 in H4.
+    subst. simpl in *. specialize (REL0 tt). pclearbot.
+    pinversion REL0; clear REL0. 2: apply ref__mono.
+    apply inj_pair2 in H2. subst. specialize (REL false). inversion REL. inversion REL0.
+  - inversion REL; clear REL.
+    apply inj_pair2 in H1.
+    apply inj_pair2 in H2.
+    apply inj_pair2 in H.
+    apply inj_pair2 in H4.
+    subst. simpl in *. specialize (REL0 tt). pclearbot.
+    pinversion REL0; clear REL0. 2: apply ref__mono.
+    apply inj_pair2 in H2. subst. specialize (REL true). inversion REL. inversion REL0.
+Qed.
